lua.v updated (except for theorem SymLua)

lua.v
@@ -119,9 +119,26 @@ Proof.
 Qed.
 
 
+Inductive LValue : LE -> Prop :=
+| LVnil : LValue LENil
+| LVnum : forall n, LValue (LENum n)
+| LVtbl : forall a, LValue (LEAddr a)
+| LVfun : forall var body, LValue (LEFun var body)
+.
+
+Inductive LExpValue : Set :=
+| LEV : forall e, LValue e -> LExpValue.
+
+
+Definition LEV2Val (me : LExpValue) :=
+  match me with
+  | LEV v _ => v
+  end.
+
+
 Inductive LMem : Set :=
 | LEmptyMem : LMem
-| LUpdate : address -> Index -> LE -> LMem -> LMem.
+| LUpdate : address -> Index -> LExpValue -> LMem -> LMem.
 
 
 Axiom LToIndex : LE -> Index.
@@ -135,7 +152,7 @@ Fixpoint Lquery (a : address) (idx : LE) (m : LMem) :=
   match m with
   | LEmptyMem => LENil
   | LUpdate a' idx' e m' => if Nat.eq_dec a a' then
-                           if Index_dec idx idx' then e
+                           if Index_dec idx idx' then (LEV2Val e)
                            else Lquery  a idx m'
                          else Lquery  a idx m'
   end.
@@ -149,7 +166,7 @@ Fixpoint Lfreshaux (m : LMem) : address :=
 
 
 Definition Lfresh (m : LMem) : (address * LMem) :=
-  let f := Lfreshaux m in (f, LUpdate f LENil LENil m).
+  let f := Lfreshaux m in (f, LUpdate f LENil (LEV LENil LVnil) m).
 
 
 Reserved Notation "'[' x ':=' s ']' t" (at level 20, x constr).
@@ -173,14 +190,6 @@ where "'[' x ':=' s ']' t" := (substitution x s t)
 .
 
 
-Inductive LValue : LE -> Prop :=
-| LVnil : LValue LENil
-| LVnum : forall n, LValue (LENum n)
-| LVtbl : forall a, LValue (LEAddr a)
-| LVfun : forall var body, LValue (LEFun var body)
-.
-
-
 Reserved Notation "m '/' e ==> m1 '/' e1"
 (at level 40, e at level 39, m1 at level 39, e1 at level 39).
 
@@ -200,8 +209,8 @@ Inductive Lstep : LMem -> LE -> LMem -> LE -> Prop :=
 | LStSet : forall m e1 m' a e2 m'' idx e3 v m''',
     m / e1 ==> m' / LEAddr a ->
     m' / e2 ==> m'' / idx ->
-    m'' / e3 ==> m''' / v ->
-    m / LESet e1 e2 e3 ==> LUpdate a idx v m''' / v
+    m'' / e3 ==> m''' / LEV2Val v ->
+    m / LESet e1 e2 e3 ==> LUpdate a idx v m''' / LEV2Val v
 | LStApp : forall m e1 var body e2 m' m'' v m''' res,
      m / e1 ==> m' / LEFun var body ->
      m' / e2 ==> m'' / v ->
@@ -228,40 +237,42 @@ Lemma L2LirValue : forall e, LValue e -> Value (Lua2Lir e).
 Proof.
   intros e HV.
   inversion HV; simpl; subst; eauto using Value.
-Qed.
+Defined.
 
 
-Definition Lmem_correct (m : LMem) := forall a n,
-    LValue (Lquery a n m) /\ LEWT MEmpty (Lquery a n m).
-
-
-Lemma Lmem_correct_update : forall m a idx e,
-  Lmem_correct m -> LEWT MEmpty e -> LValue e ->
-     Lmem_correct (LUpdate a idx e m).
-Proof.
-  unfold Lmem_correct.
-  intros.
-  split;
-  simpl;
-    destruct (Nat.eq_dec a0 a); destruct (Index_dec n idx); subst; auto;
-    apply H.
-Qed.
+Inductive Lmem_correct : LMem -> Prop :=
+| LMCE : Lmem_correct LEmptyMem
+| LMCU : forall a idx v m,
+     LEWT MEmpty (LEV2Val v) ->
+     Lmem_correct m ->
+     Lmem_correct (LUpdate a idx v m).
 
 
 Lemma mem_correct_fresh : forall m m' free,
   Lmem_correct m -> (free,m') = Lfresh m -> Lmem_correct m'.
 Proof.
   unfold Lfresh. intros m m' free Hmc Heq. inversion Heq.
-  eauto using Lmem_correct_update,LValue,LEWT.
+  eauto using Lmem_correct,LEWT.
 Qed.
 
 
-Lemma LMCquery : forall a v m, Lmem_correct m -> LValue (Lquery a v m).
-Proof. intros a v m H. apply H. Qed.
+Lemma LMCquery : forall a v m, LValue (Lquery a v m).
+Proof.
+  intros.
+  induction m; eauto using LValue.
+  destruct l. simpl.
+  breakIndexDec; trivial.
+Qed.
+
 
 
 Lemma LMCWT : forall a v m, Lmem_correct m -> LEWT MEmpty (Lquery a v m).
-Proof. intros a v m H. apply H. Qed.
+Proof.
+  intros a v m H.
+  induction H.
+  - eauto using LEWT.
+  - simpl. breakIndexDec; auto.
+Qed.
 
 
 Lemma inclusion_WT : forall Γ Γ' e,
@@ -297,8 +308,8 @@ Lemma luaPreservation : forall e m v m',
   Lmem_correct m' /\ LValue v /\ LEWT MEmpty v.
 Proof.
   intros e m v m' HM HWT HSt.
-  induction HSt; inversion HWT; subst; repeat split;
-  try apply HM; eauto using LValue;
+  induction HSt; inversion HWT; subst;
+  try (repeat split; try apply HM; eauto using LValue; fail);
   (* instantiate and split induction hyphoteses *)
   repeat match goal with
   | [ HM: Lmem_correct ?M,
@@ -312,24 +323,20 @@ Proof.
       HFr: _ = Lfresh ?M |- _ ] =>
      specialize (mem_correct_fresh _ _ _ HM HFr); clear HFr; intros
   end;
-  eauto using LValue, LEWT,Lmem_correct_update, LMCquery, LMCWT,
-              Lmem_correct_update.
-  - inversion H1; subst.
-    apply LMCquery. apply IHHSt3;
-    eauto using subst_WT.
-  - inversion H1; subst.
-    apply LMCWT. eapply IHHSt3; eauto using subst_WT.
-  - inversion H1; subst.
-    eapply IHHSt3; eauto using subst_WT.
-  - inversion H1; subst.
-    eapply IHHSt3; eauto using subst_WT.
+eauto using LValue, LEWT,Lmem_correct, LMCquery, LMCWT.
+
+  inversion H1; subst.
+  apply IHHSt3; auto.
+  apply subst_WT; auto.
+
 Qed.
 
 
 Fixpoint MLua2Lir (m : LMem) : Mem :=
   match m with
   | LEmptyMem => EmptyMem
-  | LUpdate a n e m => Update a n (Lua2Lir e) (MLua2Lir m)
+  | LUpdate a n (LEV v vv) m =>
+      Update a n (EV (Lua2Lir v) (L2LirValue v vv)) (MLua2Lir m)
   end.
 
 
@@ -339,7 +346,8 @@ Proof.
   intros Γ e.
   generalize dependent Γ.
   induction e; intros Γ HLE; inversion HLE; subst; simpl;
-  eauto 8 using IRTyping, InEq, envExt, inclusion_shadow'.
+  eauto 7 using IRTyping, eq_refl, inclusion_typing,
+    inclusion_shadow', InEq.
 Qed.
 
 
@@ -355,13 +363,16 @@ Proof.
   intros mem a idx.
   induction mem.
   - simpl. trivial.
-  - simpl. destruct (Nat.eq_dec a a0); subst; trivial.
+- destruct l. simpl. destruct (Nat.eq_dec a a0); subst; trivial.
     rewrite <- LuaIndex. destruct (Index_dec idx i); subst; trivial.
 Qed.
 
 
 Lemma L2LirFreshaux : forall m, Lfreshaux m = freshaux (MLua2Lir m).
-Proof. induction m; simpl; congruence. Qed.
+Proof.
+  induction m; trivial.
+  destruct l. simpl. congruence.
+Qed.
 
 
 Lemma L2LirFresh : forall free m m',
@@ -369,10 +380,13 @@ Lemma L2LirFresh : forall free m m',
 Proof.
   intros free m m' H.
   unfold Lfresh in H. inversion H; subst.
-  unfold fresh. f_equal.
+  unfold fresh.
+  simpl. f_equal.
   - apply L2LirFreshaux.
-  - rewrite LuaIndex. rewrite L2LirFreshaux. trivial.
+  - rewrite LuaIndex. simpl.
+    f_equal. apply L2LirFreshaux.
 Qed.
+
 
 
 Lemma L2LirSubst : forall e1 var e2,
